chore: stuff

random/TaPL/UntypedArithExp.lean
@@ -1,6 +1,3 @@
-/-- Untyped Arithmetic Expressions -/
-
-
 /-- Inductive definition of terms:
   The set of terms T contains:
   · {true, false, 0}
@@ -8,6 +5,7 @@
   · if t₁, t₂, t₃ ∈ T then "if t₁ then t₂ else t₃" ∈ T
 -/
 
+/-
 inductive newType : Nat → Type where
   | ttrue {n : Nat} : newType 0
   | ffalse {n : Nat} : newType 0
@@ -15,6 +13,21 @@ inductive newType : Nat → Type where
   | pred {n : Nat} (t : newType (n - 1)) : newType n
   | isZero {n : Nat} (t : newType (n - 1)) : newType n
   | ite {n : Nat} (t₁ t₂ t₃ : newType (n - 1)) : newType n
+-/
+
+/- Lean automatically indexes the levels of the types -/
+inductive newType : Type where
+  | ttrue : newType
+  | ffalse  : newType
+  | zero : newType
+  | pred (t : newType)  : newType
+  | isZero (t : newType) : newType
+  | ite  (t₁ t₂ t₃ : newType) : newType
+
+/- Lean generates a `sizeOf` automatically that knows the level `i` for a `tᵢ`: -/
+#reduce sizeOf newType.ttrue -- 1
+#reduce sizeOf newType.ffalse -- 1
+#reduce sizeOf (newType.isZero .ttrue) -- 2
 
 /-- Untyped Booleans -/
 
@@ -23,32 +36,49 @@ inductive t where
   | False : t
   | ite : t → t → t → t
 
-def val (i : t) : Bool :=
-  match i with
-  | t.True => true
-  | t.False => false
-  | t.ite c a b => if val c then val a else val b
+#reduce sizeOf t.True -- 1
+#reduce sizeOf t.False -- 1
+#reduce sizeOf (t.ite t.True t.True t.False) -- 4
 
-#eval val (t.True)
-#eval val (t.False)
-#eval val (t.ite t.False t.True t.False)
-#eval val (t.ite t.True t.True t.False)
-#eval val (t.ite t.True t.False t.True)
+/- define the evaluation relation: in Lean we incode it as an  *inductive prooposition* -/
 
-theorem EvalIfTrue (t₁ t₂ t₃ : t) (ht₁ : val t₁ = true) :
-    val (t.ite t₁ t₂ t₃) = val t₂ := by simp [val, ht₁]
+inductive t.EvaluatesTo : t → t → Prop
+| EvaluatesToTrue: t.EvaluatesTo (.ite .True t₂ t₃) t₂
+| EvaluatesToFalse: t.EvaluatesTo (.ite .False t₂ t₃) t₃
+| EvaluatesToIf (h : t.EvaluatesTo c c') : t.EvaluatesTo (.ite c l r) (.ite c' l r)
 
-theorem EvalIfFalse (t₁ t₂ t₃ : t) (ht₁ : val t₁ = false) :
-    val (t.ite t₁ t₂ t₃) = val t₃ := by simp [val, ht₁]
+open t
 
-theorem EvalIf (t₁ t₁' t₂ t₃ : t) (ht₁ : val t₁ = val t₁') :
-    val (t.ite t₁ t₂ t₃) = val (t.ite t₁' t₂ t₃) := by simp [val, ht₁]
+/-
+  theorem 3.5.4: determinacy of one-step evaluation
+    if t → t' and t → t'' then t' = t''
+  (note that we implement "→" as EvaluatesTo)
+-/
+theorem OneStepDeterminacy (a b c : t) (hab : t.EvaluatesTo a b) (hac : t.EvaluatesTo a c) : b = c := by
+  revert c -- need to generalize c to be able to use it afterwards in the inductive cases
+  induction hab
+  · case EvaluatesToTrue =>
+   intros c hac
+   cases hac
+   · case EvaluatesToTrue => rfl
+   · case EvaluatesToIf tthenc telsec =>
+      cases telsec -- absurd, t.True is a normal form, cannot EvaluatesTo.
+  · case EvaluatesToFalse =>
+      intros c hac
+      cases hac
+      · case EvaluatesToFalse => rfl
+      · case EvaluatesToIf tthen telse =>
+        cases telse -- absurd, t.False is a normal form, cannot EvaluatesTo.
+  · case EvaluatesToIf ac ac' al ar hacac' ih  =>
+      intros c thenRed
+      cases thenRed
+      · case EvaluatesToTrue => cases hacac' -- absurd, t.True is a normal form, cannot EvaluatesTo.
+      · case EvaluatesToFalse => cases hacac' -- absurd, t.False is a normal form, cannot EvaluatesTo.
+      · case EvaluatesToIf tthen telse =>
+          rw [ih]
+          exact telse
 
-theorem OneStepDeterminacy (t₀ t' t'' : t) (h₀ : val t₀ = val t') (h₁ : val t₀ = val t'') :
-    val t' = val t'' := by
-  cases t₀ <;> simp_all
-
-/-- Untyped Bools and Nats -/
+/--  Untyped Booleans and Naturals -/
 
 inductive t' where
   | True : t'
@@ -57,15 +87,245 @@ inductive t' where
   | zero : t'
   | succ : t' → t'
   | pred : t' → t'
-  | isZero : t' → t'
+  | iszero : t' → t'
 
+inductive t'.EvaluatesTo : t' → t' → Prop
+| -- ite true t₂ t₃ → t₂
+  EvaluatesToTrue: t'.EvaluatesTo (t'.True.ite t₂ t₃) t₂
+| -- ite false t₂ t₃ → t₃
+  EvaluatesToFalse: t'.EvaluatesTo (t'.False.ite t₂ t₃) t₃
+| -- (c → c') → (ite c l r → ite c' l r)
+  EvaluatesToIf (h : t'.EvaluatesTo c c') : (c.ite l r).EvaluatesTo (c.ite l r)
+| -- (t₁ → t₁') → (succ t₁ → succ t₂)
+  EvaluatesToSucc (h : t'.EvaluatesTo t₁ t₁') : (t'.succ t₁).EvaluatesTo (t'.succ t₁')
+| -- pred 0 = 0
+  EvaluatesToZero : (t'.pred t'.zero).EvaluatesTo (t'.zero)
+| -- pred (succ nv) → nv
+  EvaluatesToPredSucc : (t'.pred (t'.succ t₁)).EvaluatesTo  (t₁)
+| -- (t₁ → t₁') → (pred t₁ → pred t₂)
+  EvaluatesToPred (h : t'.EvaluatesTo t₁ t₁') : (t'.pred t₁).EvaluatesTo (t'.pred t₁')
+| -- iszero 0 → true
+  EvaluatesToIsZeroZero : (t'.iszero t'.zero).EvaluatesTo (t'.True)
+| -- iszero (succ nv) → false
+  EvaluatesToIsZeroSucc : (t'.iszero (t'.succ _)).EvaluatesTo (t'.False)
+| -- (t₁ → t₁') → (iszero t₁ → iszero t₂)
+  EvaluatesToIsZero (h : t'.EvaluatesTo t₁ t₁') : (t'.iszero t₁).EvaluatesTo (t'.iszero t₁')
+
+/-- exercise 3.5.14: show that theorem 3.5.4 also holds for t' -/
+theorem OneStepDeterminacy' (a b c : t') (hab : t'.EvaluatesTo a b) (hac : t'.EvaluatesTo a c) : b = c := by
+  revert c
+  induction hab
+  · -- ind. hp : (ite True t₃ t₂) → c
+    case EvaluatesToTrue t₃ t₂ =>
+      intros c cIteTrue
+      -- given the shape of cIteTrue : (t'.True.ite t₃ t₂).EvaluatesTo c
+      -- EvaluatesTo is either EvaluatesToTrue or EvaluatesToIf
+      cases cIteTrue
+      · case EvaluatesToTrue => rfl
+      · case EvaluatesToIf hEvalTrue => cases hEvalTrue
+  · -- ind. hp : (ite False t₃ t₂) → c
+    case EvaluatesToFalse t₃ t₂ =>
+      intro c cIteFalse
+      cases cIteFalse
+      · case EvaluatesToFalse => rfl
+      · case EvaluatesToIf hEvalFalse => cases hEvalFalse
+  · -- ind. hp : (ite t₁ t₃ t₂) → c
+    case EvaluatesToIf t₂ t₃ c' c hcEvalToc hcEvalToCImpc =>
+    intro c hcIte
+    -- given the shape of hcIte it can be either EvaluatesToTrue, EvaluatesToFalse, EvaluatesToIf
+    -- Lean automatically remove the non-relevant cases
+    cases hcIte
+    · case EvaluatesToTrue => cases hcEvalToc
+    · case EvaluatesToFalse => cases hcEvalToc
+    · case EvaluatesToIf c hEvaluatesTo =>
+        rw [hcEvalToCImpc]
+        exact hEvaluatesTo
+  · -- ind. hp : t₁.succ → c
+    case EvaluatesToSucc t t₁ t₁EvaluatesToT t₁EvaluatesToc =>
+    intro t t₁SuccEvalTo
+    cases t₁SuccEvalTo
+    case EvaluatesToSucc t₁ ht₁EvalTo =>
+      simp only [t'.succ.injEq]
+      exact t₁EvaluatesToc t₁ ht₁EvalTo
+  · -- ind. hp : zero.pred → c
+    case EvaluatesToZero =>
+    intro c hZeroPred
+    cases hZeroPred
+    · case EvaluatesToZero => rfl
+    · case EvaluatesToPred hZeroEvaluatesTo => cases hZeroEvaluatesTo
+  · -- ind. hp: pred (succ (t₁)) → c
+    case EvaluatesToPredSucc t₁ =>
+    -- hp : t₁.succ.pred → c
+    intro c ht₁SuccPredEvalToc
+    -- given the shape of ht₁SuccPredEvalToc,
+    -- it can be either EvaluatesToPredSucc or EvaluatesToPred
+    cases t₁.succ.pred
+    · case True =>
+        cases t₁
+        · case True =>
+            cases ht₁SuccPredEvalToc
+            · case EvaluatesToPredSucc => rfl
+            · case EvaluatesToPred hTrueEvalToPred =>
+              cases hTrueEvalToPred
+              · case EvaluatesToSucc hTrueEvalToSuccPred =>
+                cases hTrueEvalToSuccPred -- contradiction
+        · case False =>
+            cases ht₁SuccPredEvalToc
+            · case EvaluatesToPredSucc => rfl
+            · case EvaluatesToPred hFalseSuccEvalTo =>
+                cases hFalseSuccEvalTo
+                · case EvaluatesToSucc hFalseEvalToSuccPred =>
+                  cases hFalseEvalToSuccPred
+        · case ite a b c =>
+            cases ht₁SuccPredEvalToc
+            · case EvaluatesToPredSucc =>  rfl
+            · case EvaluatesToPred hIteSuccEvalTo =>
+              cases hIteSuccEvalTo
+              case EvaluatesToSucc a₁ b₁ c₁ hIteEvalTo =>
+                cases hIteEvalTo
+                · case EvaluatesToTrue =>
+
+
+                    sorry
+                · case EvaluatesToFalse =>
+                    · case True =>
+                    sorry
+                ·
+                  sorry
+        · case zero => sorry
+        · case succ u => sorry
+        · case pred u => sorry
+        · case iszero u => sorry
+    · case False =>
+        sorry
+    · case ite a b c =>
+        sorry
+    · case zero =>
+        sorry
+    · case succ u =>
+        sorry
+    · case pred u =>
+        sorry
+    · case iszero u =>
+        sorry
+  · case EvaluatesToPred t₁ t₁ t hT₁EvalToc =>
+    intro t₁ t₁PredEvalToT₁
+    -- three rules might have neen used for the reduction
+    -- however, none of the lhs of these rules overlap, meaning
+    -- that the same rule has been used to derive a → b and a → c
+    cases t₁PredEvalToT₁
+    · case EvaluatesToZero =>
+        sorry
+    · case EvaluatesToPredSucc => sorry
+    · case EvaluatesToPred t₁ t₁EvalToT₁ => sorry
+      -- exact congrArg t'.pred (hT₁EvalToc t₁ t₁EvalToT₁)
+  · case EvaluatesToIsZeroZero =>
+      intro c hZeroIsZeroEval
+      cases hZeroIsZeroEval
+      · case EvaluatesToIsZeroZero => rfl
+      · case EvaluatesToIsZero t₁ hZeroEvalTo =>
+        -- there's only one case to evaluate t'.zero
+        -- that yields t'.True = t₁.iszero
+        cases hZeroEvalTo
+  · case EvaluatesToIsZeroSucc =>
+    intro c hSuccIsZeroEval
+    cases hSuccIsZeroEval
+    · case EvaluatesToIsZeroSucc => rfl
+    · case EvaluatesToIsZero t₁ t₁' hSuccEvalTo =>
+        cases hSuccEvalTo
+        · sorry
+  · case EvaluatesToIsZero hEvalTocEq hEvalTocImp =>
+    intro c ht₁IsZeroEvalTo
+    cases ht₁IsZeroEvalTo
+    · case EvaluatesToIsZeroZero t₁ =>
+        sorry
+    · case EvaluatesToIsZeroSucc t₁ t₂ =>
+        sorry
+    · case EvaluatesToIsZero t₁ ht₁EvalTo =>
+        sorry
+
+
+/-- exercise 3.5.14: show that theorem 3.5.4 also holds for t' -/
+theorem OneStepDeterminacy'' (a b c : t') (hab : t'.EvaluatesTo a b) (hac : t'.EvaluatesTo a c) : b = c := by
+  revert c
+  induction hab
+  · -- a [EvaluatesToTrue]→ b
+    -- i.e. a = (ite true b t) [EvaluatesToTrue]→ b
+    case EvaluatesToTrue b t =>
+    intro c hIteTrueEval
+    -- let us focus on the rules that can reduce hIteTrueEval
+    cases hIteTrueEval
+    · -- either we reduce a = (ite true b t) → b
+      -- using (ite true b t) [EvaluatesToTrue] → b
+      case EvaluatesToTrue => rfl
+    · -- or we reduce a = (ite true b t) → b
+      -- using (ite true b t) [EvaluatesToIf] → a'.ite b t
+      -- under the hypothesis that true → a'
+      case EvaluatesToIf a' hTrueEvalToa' =>
+        -- we now study the reduction of true → a'
+        -- the only rule that allows for this reduction is: true [EvaluatesToTrue] → a'
+        -- however, this reduction is absurd, since true (t'.True) is in NF already!
+        -- in fact, no evaluation rule can reduce t'.True to anything.
+        cases hTrueEvalToa'
+  · -- a [EvaluatesToFalse]→ b
+    -- i.e. a = (ite false b t) [EvaluatesToFalse]→ b
+    case EvaluatesToFalse t c =>
+    intro c hIteFalseEval
+    -- we study hIteFalseEval
+    cases hIteFalseEval
+    · -- (ite false t c) [EvaluatesToFalse] → c
+      case EvaluatesToFalse => rfl
+    · -- (ite false t c) [EvaluatesToIf] → c
+      -- required hypothesis false [EvaluatesTo?]→ c, which is absurd
+      case EvaluatesToIf a' hFalseEvalToa' =>
+        cases hFalseEvalToa'
+  · -- a [EvaluatesToIf]→ b
+    -- i.e. a [EvaluatesToIf] → b
+    -- in this case, we know that b will be something like b = ite b1 a2 a3
+    -- and given a = ite a1 a2 a3, to have a [EvaluatesToIf] → b we need a1 → b1
+    case EvaluatesToIf a b a2 a3 ha1EvalTob1 ha1EvalTocImp =>
+    -- ha1EvalTocImp : ∀ (c : t'), a.EvaluatesTo c → b = c
+    -- is the inductive hypothesis (a [EvaluatesTo]→ c) → b = c
+    -- note that we are supposing already that a [EvaluatesToIf]→ b
+    intro c hIteEval
+    -- we study the reductions that apply to hIteEval
+    -- under the hypotheses that
+    -- (1) (a → c) → b = c
+    -- (2) a → b
+    -- given the hypothesis
+    cases hIteEval
+    · -- if (ite a1 a2 a3) [EvaluatesToTrue]→ c
+      -- and by (2) we know (a1 → b) [EvaluatesToIf]→ ((ite a1 a2 a3) → (ite b a2 a3))
+      -- then we require a1 → true, and already b1 → true, thus true → b1 which is absurd
+      case EvaluatesToTrue => cases ha1EvalTob1
+    ·
+      sorry
+    ·
+      sorry
+  · sorry
+  · sorry
+  · sorry
+  · sorry
+  · sorry
+  · sorry
+  · sorry
+
+/-
+/-- Untyped Bools and Nats -/
+inductive t' where
+  | True : t'
+  | False : t'
+  | ite : t' → t' → t' → t'
+  | zero : t'
+  | succ : t' → t'
+  | pred : t' → t'
+  | isZero : t' → t'
 def valB (b : t') :=
   match b with
   | t'.True => true
   | t'.False => false
   | t'.ite c a b => if valB c then valB a else valB b
   | _ => sorry
-
 def valN (n : t') : Nat :=
   match n with
   | t'.True => valB n
@@ -75,3 +335,4 @@ def valN (n : t') : Nat :=
   | t'.succ => val: t' → t'
   | t'.pred => val: t' → t'
   | t'.isZero => val: t' → t'
+-/
